Adding a new function/lambda expander

books/projects/smtlink/verified/expand-cp.lisp
@@ -9,866 +9,318 @@
 (include-book "std/util/bstar" :dir :system)
 (include-book "xdoc/top" :dir :system)
 (include-book "std/util/define" :dir :system)
-;; for symbol-fix
-(include-book "centaur/fty/basetypes" :dir :system)
-;; for symbol-list-fix
-(include-book "centaur/fty/baselists" :dir :system)
-(include-book "centaur/misc/hons-extra" :dir :system)
+(include-book "centaur/fty/top" :dir :system)
 ;; To be compatible with Arithmetic books
-(include-book "ordinals/lexicographic-ordering-without-arithmetic" :dir :system)
-;; Meta-extract stuff
-(include-book "clause-processors/just-expand" :dir :system)
+(include-book "ordinals/lexicographic-ordering-without-arithmetic" :dir
+              :system)
+(include-book "clause-processors/meta-extract-user" :dir :system)
+(include-book "clause-processors/unify-subst" :dir :system)
 
-;; Include SMT books
-(include-book "generalize")
+(include-book "../utils/pseudo-term")
+(include-book "../utils/fresh-vars")
+(include-book "hint-interface")
+(include-book "basics")
 
 (set-state-ok t)
 
-(defsection function-expansion
-  :parents (verified)
-  :short "Function expansion"
+(defalist sym-int-alist
+  :key-type symbolp
+  :val-type integerp
+  :true-listp t
+  :pred sym-int-alistp)
 
-  (defalist sym-nat-alist
-    :key-type symbol
-    :val-type natp
-    :pred sym-nat-alistp
-    :true-listp t)
+(defthm assoc-equal-of-sym-int-alist
+  (implies (and (sym-int-alistp y)
+                (assoc-equal x y))
+           (and (consp (assoc-equal x y))
+                (integerp (cdr (assoc-equal x y))))))
 
+(defalist pseudo-term-sym-alist
+  :key-type pseudo-termp
+  :val-type symbolp
+  :true-listp t
+  :pred pseudo-term-sym-alistp)
+
+(defthm assoc-equal-of-pseudo-term-sym-alist
+  (implies (and (pseudo-term-sym-alistp y)
+                (assoc-equal x y))
+           (and (consp (assoc-equal x y))
+                (symbolp (cdr (assoc-equal x y))))))
+
+(defthm crock
+  (implies (symbolp x) (pseudo-termp x)))
+
+(define new-vars-for-actuals ((actuals pseudo-term-listp)
+                              (alst pseudo-term-sym-alistp)
+                              (names symbol-listp))
+  :measure (len (pseudo-term-list-fix actuals))
+  :returns (mv (vars pseudo-term-listp)
+               (new-alst pseudo-term-sym-alistp)
+               (new-names symbol-listp))
+  (b* ((actuals (pseudo-term-list-fix actuals))
+       (alst (pseudo-term-sym-alist-fix alst))
+       (names (symbol-list-fix names))
+       ((unless (consp actuals))
+        (mv nil alst names))
+       ((cons ac-hd ac-tl) actuals)
+       ((mv new-ac-tl alst-1 names-1)
+        (new-vars-for-actuals ac-tl alst names))
+       ((if (or (acl2::variablep ac-hd)
+                (acl2::fquotep ac-hd)))
+        (mv (cons ac-hd new-ac-tl) alst-1 names-1))
+       (new-var (new-fresh-var names)))
+    (mv (cons new-var new-ac-tl)
+        (acons ac-hd new-var alst-1)
+        (cons new-var names-1))))
+
+(encapsulate ()
   (local
-   (defthm consp-of-sym-nat-alist-fix
-     (implies (consp (sym-nat-alist-fix x)) (consp x))
-     :hints (("Goal" :in-theory (enable sym-nat-alist-fix))))
-   )
+   (in-theory (disable assoc-equal lambda-of-pseudo-lambdap
+                       symbol-listp)))
 
+(define get-formals-body ((fn symbolp)
+                          state)
+  :returns (mv (formals symbol-listp)
+               (body pseudo-termp))
+  (b* ((fn (symbol-fix fn))
+       (formula (acl2::meta-extract-formula-w fn (w state)))
+       ((unless (pseudo-termp formula))
+        (prog2$
+         (er hard? 'expand-cp=>get-formals-body
+             "Formula got by meta-extract ~p0 is not a pseudo-termp." fn)
+         (mv nil nil)))
+       ((mv ok lhs rhs)
+        (case-match formula
+          (('equal lhs rhs)
+           (mv t lhs rhs))
+          (& (mv nil nil nil))))
+       ((unless (and ok (consp lhs) (symbol-listp (cdr lhs))))
+        (prog2$ (er hard? 'expand-cp=>get-formals-body
+                    "Malformed function definition formula: ~p0~%" formula)
+                (mv nil nil))))
+    (mv (cdr lhs) rhs)))
+)
+
+(define update-fn-lvls ((fn symbolp)
+                        (fn-info maybe-smt-function-p)
+                        (fn-lvls sym-int-alistp))
+  :returns (new-lvls
+            sym-int-alistp
+            :hints (("Goal"
+                     :in-theory (disable assoc-equal-of-sym-int-alist)
+                     :use ((:instance assoc-equal-of-sym-int-alist
+                                      (x (symbol-fix fn))
+                                      (y (sym-int-alist-fix fn-lvls)))))))
+  (b* ((fn (symbol-fix fn))
+       (fn-info (maybe-smt-function-fix fn-info))
+       (fn-lvls (sym-int-alist-fix fn-lvls))
+       (lvl (assoc-equal fn fn-lvls))
+       ((if lvl) (acons fn (1- (cdr lvl)) fn-lvls))
+       ((if fn-info)
+        (acons fn (1- (smt-function->expansion-depth fn-info)) fn-lvls)))
+    (acons fn 0 fn-lvls)))
+
+(encapsulate ()
   (local
-   (defthm len-of-sym-nat-alist-fix-<
-     (> (1+ (len x)) (len (sym-nat-alist-fix x)))
-     :hints (("Goal" :in-theory (enable sym-nat-alist-fix))))
-   )
+   (in-theory (disable symbolp-of-fn-call-of-pseudo-termp
+                       pseudo-term-listp-of-symbol-listp
+                       acl2::symbol-listp-when-not-consp
+                       acl2::pseudo-termp-opener
+                       pairlis$
+                       acl2::pseudo-term-listp-cdr
+                       pseudo-term-listp-of-cdr-pseudo-termp-if
+                       default-car
+                       acl2::pseudo-lambdap-of-car-when-pseudo-lambda-listp
+                       acl2::true-listp-of-car-when-true-list-listp
+                       true-list-listp
+                       (:executable-counterpart smt-basics))))
 
-  (local
-   (defthm natp-of-cdar-sym-nat-alist-fix
-     (implies (consp (sym-nat-alist-fix x))
-              (natp (cdar (sym-nat-alist-fix x))))
-     :hints (("Goal" :in-theory (enable sym-nat-alist-fix))))
-   )
+(defines expand-term
+  :well-founded-relation l<
+  :flag-local nil
+  :verify-guards nil
+  :hints (("Goal"
+           :in-theory (disable pseudo-termp
+                               pseudo-term-listp)))
 
-  (define update-fn-lvls ((fn symbolp) (fn-lvls sym-nat-alistp))
-    :returns (updated-fn-lvls sym-nat-alistp)
-    :measure (len fn-lvls)
-    :hints (("Goal" :in-theory (enable sym-nat-alist-fix)))
-    (b* ((fn (symbol-fix fn))
-         (fn-lvls (sym-nat-alist-fix fn-lvls))
-         ((unless (consp fn-lvls)) nil)
-         ((cons first rest) fn-lvls)
-         ((cons this-fn this-lvl) first)
-         ((unless (equal fn this-fn))
-          (cons (cons this-fn this-lvl)
-                (update-fn-lvls fn rest))))
-      (if (zp this-lvl)
-          (cons (cons this-fn 0) rest)
-        (cons (cons this-fn (1- this-lvl)) rest)))
-    ///
-    (more-returns
-     (updated-fn-lvls
-      (implies (and (symbolp fn)
-                    (sym-nat-alistp fn-lvls)
-                    (consp fn-lvls)
-                    (assoc-equal fn fn-lvls)
-                    (not (equal (cdr (assoc-equal fn fn-lvls)) 0)))
-               (< (cdr (assoc fn updated-fn-lvls))
-                  (cdr (assoc fn fn-lvls))))
-      :name updated-fn-lvls-decrease))
-    )
-
-
-  ;; val-type can be a list of pseudo-termp
-  ;; This will give us two benefits: multiple facts and when it's nil,
-  ;; fact-finder fails to find a fact.
-  (defalist fact-alist
-    :key-type pseudo-termp
-    :val-type pseudo-termp
-    :pred fact-alistp
-    :short "Value is the equivalence term about Key term."
-    :true-listp t)
-
-  (defprod ex-args
-    :parents (function-expansion)
-    :short "Argument list for function expand"
-    ((fn-lvls sym-nat-alistp "Levels to expand each functions to."
-              :default nil)
-     (fn-lst smt-function-list-p "List of function definitions to use for
-      function expansion." :default nil)
-     (facts fact-alistp "An alist of current learnt equivalence facts."
-            :default nil)
-     (fixinfo smt-fixtype-info-p "FTY information." :default nil)
-     (wrld-fn-len natp "Number of function definitions in curent world."
-                  :default 0)))
-
-  (local
-   (defthm natp-of-sum-lvls-lemma
-     (implies (and (consp (sym-nat-alist-fix fn-lvls)) (natp x))
-              (natp (+ (cdr (car (sym-nat-alist-fix fn-lvls))) x)))
-     :hints (("Goal"
-              :in-theory (enable sym-nat-alist-fix)
-              :use ((:instance natp-of-cdar-sym-nat-alist-fix)))))
-   )
-
-  (define sum-lvls ((fn-lvls sym-nat-alistp))
-    :returns
-    (sum natp
-         :hints (("Goal"
-                  :use ((:instance
-                         natp-of-sum-lvls-lemma
-                         (x (sum-lvls (cdr (sym-nat-alist-fix fn-lvls)))))))))
-    :measure (len fn-lvls)
-    :hints (("Goal" :in-theory (enable sym-nat-alist-fix)))
-    (b* ((fn-lvls (sym-nat-alist-fix fn-lvls))
-         ((unless (consp fn-lvls)) 0)
-         ((cons first rest) fn-lvls)
-         ((cons & lvl) first))
-      (+ lvl (sum-lvls rest)))
-    ///
-    (defthm sum-lvls-decrease-after-update
-      (implies (and (symbolp fn)
-                    (sym-nat-alistp fn-lvls)
-                    (consp fn-lvls)
-                    (assoc-equal fn fn-lvls)
-                    (not (equal (cdr (assoc-equal fn fn-lvls)) 0)))
-               (< (sum-lvls (update-fn-lvls fn fn-lvls))
-                  (sum-lvls fn-lvls)))
-      :hints (("Goal" :in-theory (enable update-fn-lvls)))))
-
-  (define function-substitution ((term pseudo-termp)
-                                 state)
-    :returns (subst-term
-              pseudo-termp
-              :hints (("Goal"
-                       :in-theory (e/d ()
-                                       (pseudo-termp
-                                        pseudo-term-listp
-                                        acl2::return-type-of-substitute-into-term.xx
-                                        acl2::return-type-of-simple-one-way-unify.a))
-                       :use ((:instance
-                              acl2::return-type-of-simple-one-way-unify.a
-                              (pat (cadr (acl2::meta-extract-formula-w
-                                          (symbol-fix fn-call)
-                                          (cdr (assoc-equal 'acl2::current-acl2-world
-                                                            (nth 2 state))))))
-                              (term (pseudo-term-fix term))
-                              (alist nil))))))
-    :guard-hints (("Goal"
-                   :in-theory (disable symbol-listp assoc-equal)))
-    (b* ((term (pseudo-term-fix term))
-         ((unless (and (not (acl2::variablep term))
-                       (not (acl2::fquotep term))
-                       (symbolp (car term))))
-          (prog2$
-           (er hard? 'expand-cp=>function-substitution "expand-cp: fn-call is nil
-                               or 'quote.")
-           nil))
-         ((cons fn-call &) term)
-         (formula (acl2::meta-extract-formula-w fn-call (w state)))
-         ((unless (pseudo-termp formula))
-          (prog2$
-           (er hard? 'expand-cp=>function-substitution "expand-cp: formula got by
-       meta-extract ~p0 is not a pseudo-termp." fn-call)
-           nil))
-         ((mv ok lhs rhs)
-          (case-match formula
-            (('equal lhs rhs)
-             (mv t lhs rhs))
-            (& (mv nil nil nil))))
-         ((unless (and ok (pseudo-termp lhs)))
-          (prog2$ (er hard? 'expand-cp=>function-substitution "expand-cp: formula got by
-       meta-extract ~p0 is not an equality." fn-call)
-                  nil))
-         ((mv match-ok subst)
-          (acl2::simple-one-way-unify lhs term nil))
-         ((unless match-ok)
-          (prog2$
-           (er hard? 'expand-cp=>function-substitution "expand-cp:
-       simple-one-way-unify failed.")
-           nil)))
-      `(equal ,term ,(acl2::substitute-into-term rhs subst))))
-
-  (encapsulate()
-    (local (in-theory (e/d (function-substitution) (w))))
-
-    (defthm function-substitution-correct
-      (implies (and (ev-smtcp-meta-extract-global-facts)
-                    (pseudo-termp term)
-                    (alistp a)
-                    (function-substitution term state))
-               (ev-smtcp (function-substitution term state) a))
-      :hints (("Goal"
-               :in-theory (e/d ()
-                               (ev-smtcp-meta-extract-formula))
-               :use ((:instance
-                      ev-smtcp-meta-extract-formula
-                      (name (car term))
-                      (st state)
-                      (a (ev-smtcp-alist
-                          (mv-nth 1
-                                  (acl2::simple-one-way-unify
-                                   (cadr (meta-extract-formula (car term) state))
-                                   term nil))
-                          a)))))))
-    )
-
-  (encapsulate ()
-    (local
-     (defthm type-of-assoc-equal-of-sym-nat-alistp
-       (implies (and (sym-nat-alistp x)
-                     (symbolp y)
-                     (assoc-equal y x))
-                (and (symbolp (car (assoc-equal y x)))
-                     (natp (cdr (assoc-equal y x))))))
-     )
-
-    (define fact-finder ((term pseudo-termp)
-                         (expand-args ex-args-p)
+  (define expand-lambda ((term pseudo-termp)
+                         (hints smtlink-hint-p)
+                         (fn-lvls sym-int-alistp)
+                         (alst pseudo-term-sym-alistp)
+                         (clock natp)
+                         (names symbol-listp)
                          state)
-      :guard (and (not (acl2::variablep term))
-                  (not (acl2::fquotep term))
-                  (symbolp (car term))
-                  (not (assoc-equal term (ex-args->facts expand-args)))
-                  (not (zp (ex-args->wrld-fn-len expand-args))))
-      :guard-hints (("Goal"
-                     :in-theory (e/d ()
-                                     (type-of-assoc-equal-of-sym-nat-alistp))
-                     :use ((:instance type-of-assoc-equal-of-sym-nat-alistp
-                                      (x (ex-args->fn-lvls expand-args))
-                                      (y (car term))))))
-      :returns (mv (new-term pseudo-termp)
-                   (new-args ex-args-p))
-      :short "Find the definition fact for @('term')"
-      :long "<p>Given a pseudo-termp @('term') that is not a @('variablep'), not
-a @('fquotep'), nor a @('pseudo-lambdap'), and that it doesn't exist in the
-list of facts learnt @('(ex-args->facts expand-args)'), we want to find the
-definition fact of that term.</p>
-"
-      (b* ((term (pseudo-term-fix term))
-           (expand-args (ex-args-fix expand-args))
-           ((ex-args a) expand-args)
-           ((cons fn &) term)
-           ;; There are three cases:
-           ;; 1. fn is a basic function (including fty functions) -- fn-lvls stays
-           ;; the same, nothing is expanded, no fact generated
-           ;; For 2 and 3, if fn-lvls is already 0, then do nothing; if fn-lvls is
-           ;; not 0, expand.
-           ;; 2. fn exists in user-defined fn-lvls -- fn-lvls decrease by 1, fn is
-           ;; expanded, one fact generated
-           ;; 3. otherwise, fn will be expanded once -- fn-lvls decrease by 1, fn
-           ;; is expanded, one fact generated
-           (basic-function (member-equal fn *SMT-basics*))
-           (flex? (fncall-of-fixtypes fn a.fixinfo))
-           ((if (or basic-function flex?))
-            (mv nil a))
-           (lvl (assoc-equal fn a.fn-lvls))
-           (user-defined (is-function fn a.fn-lst))
-           ((if (and lvl (zp (cdr lvl)) user-defined)) (mv nil a))
-           ((if (and lvl (zp (cdr lvl)) (null user-defined)))
-            (prog2$ (er hard? 'expand-cp=>fact-finder "Possibly
-                       encountered recursive functions that are not
-                       user-defined: ~q0" term)
-                    (mv nil a)))
-           (fact (function-substitution term state))
-           ((if (null fact)) (mv nil a))
-           ((if lvl)
-            (mv fact
-                (make-ex-args :fn-lvls (update-fn-lvls fn a.fn-lvls)
-                              :fn-lst a.fn-lst
-                              :facts (acons term fact a.facts)
-                              :fixinfo a.fixinfo
-                              :wrld-fn-len a.wrld-fn-len))))
-        ;; if not in fn-lvls
-        (mv fact
-            (make-ex-args :fn-lst a.fn-lst
-                          :fn-lvls (cons `(,fn . 0) a.fn-lvls)
-                          :facts (acons term fact a.facts)
-                          :fixinfo a.fixinfo
-                          :wrld-fn-len (1- a.wrld-fn-len))))
-      ///
-      (more-returns
-       (new-args
-        (implies
-         (and (pseudo-termp term)
-              (ex-args-p expand-args)
-              (symbolp (car term))
-              new-term
-              (assoc-equal (car term)
-                           (ex-args->fn-lvls expand-args)))
-         (and (< (sum-lvls (ex-args->fn-lvls new-args))
-                 (sum-lvls (ex-args->fn-lvls expand-args)))
-              (equal (ex-args->wrld-fn-len new-args)
-                     (ex-args->wrld-fn-len expand-args))))
-        :hints (("Goal"
-                 :in-theory (e/d ()
-                                 (sum-lvls-decrease-after-update))
-                 :use ((:instance sum-lvls-decrease-after-update
-                                  (fn (car term))
-                                  (fn-lvls (ex-args->fn-lvls expand-args))))))
-        :name fact-finder-decrease-1)
-       (new-args
-        (implies
-         (and (pseudo-termp term)
-              (ex-args-p expand-args)
-              (symbolp (car term))
-              (not (zp (ex-args->wrld-fn-len expand-args)))
-              new-term
-              (not (assoc-equal (car term)
-                                (ex-args->fn-lvls expand-args))))
-         (< (ex-args->wrld-fn-len new-args)
-            (ex-args->wrld-fn-len expand-args)))
-        :name fact-finder-decrease-2)
-       (new-args
-        (implies (not new-term)
-                 (and (equal (ex-args->wrld-fn-len new-args)
-                             (ex-args->wrld-fn-len expand-args))
-                      (equal (sum-lvls (ex-args->fn-lvls new-args))
-                             (sum-lvls (ex-args->fn-lvls expand-args)))))
-        :name fact-finder-same-3)))
-    )
-
-  (encapsulate ()
-    (local
-     (defthm acl2-count-of-last-of-consp-decrease
-       (implies (consp x)
-                (< (acl2-count (pseudo-term-fix (car (last x))))
-                   (acl2-count x)))
-       :hints (("Goal"
-                :in-theory (enable pseudo-term-fix)))
-       ))
-
-    (defines transform
-      :well-founded-relation l<
-      :flag-local nil
-      :flag-defthm-macro defthm-transform
-      :verify-guards nil
-
-      (define transform-list ((term-lst pseudo-term-listp))
-        :returns (new-term-lst pseudo-term-listp)
-        :measure (acl2-count (pseudo-term-list-fix term-lst))
-        (b* ((term-lst (pseudo-term-list-fix term-lst))
-             ((unless (consp term-lst)) term-lst)
-             ((cons first rest) term-lst)
-             (first-term (transform first)))
-          (cons first-term
-                (transform-list rest))))
-
-      (define transform ((term pseudo-termp))
-        :returns (new-term pseudo-termp)
-        :measure (acl2-count (pseudo-term-fix term))
-        :hints (("Goal"
-                 :in-theory (e/d ()
-                                 (acl2-count-of-last-of-consp-decrease))
-                 :use ((:instance acl2-count-of-last-of-consp-decrease
-                                  (x (cdr (pseudo-term-fix term)))))))
-        (b* ((term (pseudo-term-fix term))
-             ;; If first term is a symbolp or is quoted, return the current facts
-             ((if (or (acl2::variablep term) (acl2::fquotep term))) term)
-             ;; The first term is now a function call:
-             ;; Cons the function call and function actuals out of term
-             ((cons fn-call fn-actuals) term)
-             ;; If fn-call is a pseudo-lambdap, transform the body
-             ((if (pseudo-lambdap fn-call))
-              (b* (((list 'lambda formal-lst body) fn-call)
-                   (transformed-body (transform body))
-                   (transformed-actuals (transform-list fn-actuals)))
-                (lambda-substitution `(lambda ,formal-lst
-                                        ,transformed-body)
-                                     transformed-actuals)))
-             ;; If fn-call is neither a lambda expression nor a function call
-             ((unless (mbt (symbolp fn-call))) nil)
-
-             ;; -----------------------------------------------------------
-             ;; Now the term is a function call
-             ((if (and (equal fn-call 'acl2::return-last)
-                       (equal (len fn-actuals) 3)))
-              (transform (car (last term)))))
-          (cons fn-call (transform-list fn-actuals))))
-      )
-
-    (local
-     (defthm tranform-list-maintain-length
-       (implies (pseudo-term-listp term-lst)
-                (equal (len (transform-list term-lst))
-                       (len term-lst)))
-       :hints (("Goal"
-                :expand (transform-list term-lst))))
-     )
-
-    (local
-     (defthm pseudo-lambdap-of-reconstruction
-       (implies (and (pseudo-termp term)
-                     (consp term)
-                     (not (equal 'quote (car term)))
-                     (pseudo-lambdap (car term)))
-                (pseudo-lambdap (list 'lambda
-                                      (cadr (car term))
-                                      (transform (caddr (car term))))))
-       :hints (("Goal"
-                :in-theory (e/d (pseudo-lambdap)
-                                (symbol-listp
-                                 pseudo-term-listp-of-cdr-of-pseudo-termp
-                                 pseudo-term-listp
-                                 pseudo-term-listp-of-symbol-listp))))))
-
-    (local
-     (defthm pseudo-termp-of-car-of-last-of-return-last
-       (implies (and (pseudo-term-listp x)
-                     (consp x))
-                (pseudo-termp (car (last x))))
-       :hints (("Goal"
-                :in-theory (enable pseudo-term-listp last)))
-       ))
-
-    (verify-guards transform)
-
-    (defines induction-scheme
-      :well-founded-relation l<
-      :flag-local nil
-      :verify-guards nil
-
-      (define induction-scheme-list ((term-lst pseudo-term-listp)
-                                     (al))
-        (declare (irrelevant al))
-        :measure (acl2-count (pseudo-term-list-fix term-lst))
-        (b* ((term-lst (pseudo-term-list-fix term-lst))
-             ((unless (consp term-lst)) term-lst)
-             ((cons first rest) term-lst))
-          (cons (induction-scheme first al)
-                (induction-scheme-list rest al))))
-
-      (define induction-scheme ((term pseudo-termp)
-                                (al))
-        (declare (irrelevant al))
-        :measure (acl2-count (pseudo-term-fix term))
-        :hints (("Goal"
-                 :in-theory (e/d ()
-                                 (acl2-count-of-last-of-consp-decrease
-                                  symbol-listp
-                                  acl2::pseudo-lambdap-of-car-when-pseudo-termp
-                                  consp-of-sym-nat-alist-fix
-                                  sym-nat-alist-fix-when-sym-nat-alistp))
-                 :use ((:instance acl2-count-of-last-of-consp-decrease
-                                  (x (cdr (pseudo-term-fix term)))))))
-        (b* ((term (pseudo-term-fix term))
-             ;; If first term is a symbolp or is quoted, return the current facts
-             ((if (or (acl2::variablep term) (acl2::fquotep term))) term)
-             ;; The first term is now a function call:
-             ;; Cons the function call and function actuals out of term
-             ((cons fn-call fn-actuals) term)
-             ;; If fn-call is a pseudo-lambdap, transform the body
-             ((if (pseudo-lambdap fn-call))
-              (b* (((list 'lambda formal-lst body) fn-call)
-                   ;; (transformed-body (transform body))
-                   ;; (transformed-actuals (transform-list fn-actuals)))
-                   )
-                (lambda-substitution
-                 (induction-scheme body
-                                   (pairlis$ formal-lst
-                                             (ev-smtcp-lst fn-actuals al)))
-                 (induction-scheme-list fn-actuals al))))
-             ;; If fn-call is neither a lambda expression nor a function call
-             ((unless (mbt (symbolp fn-call))) nil)
-
-             ;; -----------------------------------------------------------
-             ;; Now the term is a function call
-             ((if (and (equal fn-call 'acl2::return-last)
-                       (equal (len fn-actuals) 3)))
-              (induction-scheme (car (last term)) al)))
-          (induction-scheme-list fn-actuals al)))
-      )
-
-    (local
-     (defthm induction-scheme-list-maintain-length
-       (implies (pseudo-term-listp term-lst)
-                (equal (len (induction-scheme-list term-lst al))
-                       (len term-lst)))
-       :hints (("Goal"
-                :expand ((induction-scheme-list term-lst al)
-                         (induction-scheme-list nil al)))))
-     )
-
-    (local
-     (defthm cdr-of-transform-list
-       (implies (pseudo-term-listp x)
-                (equal (transform-list (cdr x))
-                       (cdr (transform-list x))))
-       :hints (("Goal"
-                :expand (transform-list x)))
-       ))
-
-    (local
-     (defthm crock1
-       (implies (equal (len x) 1)
-                (equal (car (last x))
-                       (car x)))
-       :hints (("Goal"
-                :in-theory (enable last len)))))
-
-    (defthm-induction-scheme-flag
-      (defthm transform-pseudo-termp
-        (implies (and (ev-smtcp-meta-extract-global-facts)
-                      (pseudo-termp term)
-                      (alistp a))
-                 (equal (ev-smtcp (transform term) a)
-                        (ev-smtcp term a)))
-        :hints ('(:expand ((transform term))
-                          :in-theory (e/d (ev-smtcp-of-fncall-args)
-                                          (lambda-substitution
-                                           symbol-listp
-                                           acl2::symbolp-of-car-when-symbol-listp
-                                           acl2::symbol-listp-of-cdr-when-symbol-listp
-                                           acl2::true-listp-of-car-when-true-list-listp
-                                           true-list-listp))))
-        :flag induction-scheme)
-      (defthm transform-pseudo-term-listp
-        (implies (and (ev-smtcp-meta-extract-global-facts)
-                      (pseudo-term-listp term-lst)
-                      (alistp a))
-                 (equal (ev-smtcp-lst (transform-list term-lst) a)
-                        (ev-smtcp-lst term-lst a)))
-        :hints ('(:expand ((transform-list term-lst)
-                           (transform-list nil))))
-        :flag induction-scheme-list)
-      :hints(("Goal" :induct (induction-scheme-flag flag term-lst term a))))
-
-    (defthm transform-implies-function-substitution
-      (implies (and (pseudo-termp term)
-                    (transform (function-substitution term state)))
-               (function-substitution term state))
-      :hints (("Goal"
-               :in-theory (e/d (transform)
-                               ()))))
-
-    (defthm transform-function-substitution-correct
-      (implies (and (ev-smtcp-meta-extract-global-facts)
-                    (pseudo-termp term)
-                    (alistp a)
-                    (transform (function-substitution term state)))
-               (ev-smtcp (transform (function-substitution term state)) a))
-      :hints (("Goal"
-               :in-theory (e/d (transform) ()))))
-
-    (defines expand
-      :well-founded-relation l<
-      :flag-local nil
-      :verify-guards nil
-      :flag-defthm-macro defthm-expand
-      :hints (("Goal"
-               :in-theory (e/d ()
-                               (fact-finder-decrease-1
-                                fact-finder-decrease-2
-                                fact-finder-same-3
-                                pseudo-termp
-                                symbol-listp
-                                pseudo-term-listp-of-symbol-listp
-                                consp-of-sym-nat-alist-fix
-                                pseudo-term-listp
-                                acl2::pseudo-termp-opener
-                                rational-listp
-                                integer-listp))
-               :use ((:instance fact-finder-decrease-1
-                                (term (pseudo-term-fix term))
-                                (expand-args (ex-args-fix expand-args)))
-                     (:instance fact-finder-decrease-2
-                                (term (pseudo-term-fix term))
-                                (expand-args (ex-args-fix expand-args)))
-                     (:instance fact-finder-same-3
-                                (term (pseudo-term-fix term))
-                                (expand-args (ex-args-fix expand-args)))
-                     (:instance acl2-count-of-last-of-consp-decrease
-                                (x (cdr (pseudo-term-fix term))))
-                     )))
-
-      (define expand-list ((term-lst pseudo-term-listp)
-                           (expand-args ex-args-p)
-                           state)
-        :returns (fact-alst fact-alistp)
-        :measure (list (ex-args->wrld-fn-len expand-args)
-                       (sum-lvls (ex-args->fn-lvls expand-args))
-                       (acl2-count (pseudo-term-list-fix term-lst)))
-        (b* ((term-lst (pseudo-term-list-fix term-lst))
-             (expand-args (ex-args-fix expand-args))
-             ((ex-args a) expand-args)
-             ((unless (consp term-lst)) a.facts)
-             ((cons first rest) term-lst)
-             (facts-first (expand first a state)))
-          (expand-list rest (change-ex-args a :facts facts-first) state)))
-
-      (define expand ((term pseudo-termp)
-                      (expand-args ex-args-p)
-                      state)
-        :returns (fact-alst fact-alistp)
-        :measure (list (ex-args->wrld-fn-len expand-args)
-                       (sum-lvls (ex-args->fn-lvls expand-args))
-                       (acl2-count (pseudo-term-fix term)))
-        (b* ((term (pseudo-term-fix term))
-             (expand-args (ex-args-fix expand-args))
-             ((ex-args a) expand-args)
-             ((if (zp a.wrld-fn-len)) a.facts)
-             ;; If first term is a symbolp or is quoted, return the current facts
-             ((if (or (acl2::variablep term) (acl2::fquotep term))) a.facts)
-             ;; The first term is now a function call:
-             ;; Cons the function call and function actuals out of term
-             ((cons fn-call fn-actuals) term)
-             ;; If fn-call is a pseudo-lambdap, substitute unbounded variables in the
-             ;; lambda and recurse to expand the substituted term.
-             ;; To ensure termination, wrld-fn-len needs to decrease, this means
-             ;; wrld-fn-len should include term size so that it's large enough.
-             ((if (pseudo-lambdap fn-call))
-              (expand (lambda-substitution fn-call fn-actuals)
-                      (change-ex-args a :wrld-fn-len (1- a.wrld-fn-len))
-                      state))
-             ;; If fn-call is neither a lambda expression nor a function call
-             ((unless (mbt (symbolp fn-call))) nil)
-
-             ;; -----------------------------------------------------------
-             ;; Now the term is a function call
-             ;; if fn-call is return-last, we can skill the term
-             ((if (equal fn-call 'acl2::return-last)) a.facts)
-             ;; we first test if term already exists in facts alist.
-             (exists? (assoc-equal term a.facts))
-             ;; I can skip the whole subtree because if such a term already exists in
-             ;; facts, then it's subterms, subsubterms ... must also exist in the
-             ;; facts. This is because we are doing a depth first travesal.
-             ((if exists?) a.facts)
-             ((mv new-term new-args) (fact-finder term a state))
-             ;; new-term being nil meaning there's no fact to prove
-             ((unless new-term)
-              (expand-list fn-actuals new-args state)))
-          (expand new-term new-args state)))
-      )
-
-    (verify-guards expand)
-    )
-
-  (define initialize-fn-lvls ((fn-lst smt-function-list-p))
-    :returns (fn-lvls sym-nat-alistp)
-    :measure (len fn-lst)
-    (b* ((fn-lst (smt-function-list-fix fn-lst))
-         ((unless (consp fn-lst)) nil)
-         ((cons first rest) fn-lst)
-         ((smt-function f) first))
-      (cons (cons f.name f.expansion-depth) (initialize-fn-lvls rest))))
-
-  (define generate-type ((term pseudo-termp)
-                         (fn-lst smt-function-list-p)
-                         state)
-    :returns (new-term pseudo-termp)
+    :guard (and (consp term)
+                (pseudo-lambdap (car term))
+                (not (zp clock)))
+    :measure (list (nfix clock)
+                   (acl2-count (pseudo-term-fix term))
+                   1)
+    :returns (mv (new-term pseudo-termp)
+                 (new-alst pseudo-term-sym-alistp)
+                 (new-names symbol-listp))
     (b* ((term (pseudo-term-fix term))
-         (fn-lst (smt-function-list-fix fn-lst))
-         ((unless (consp term))
-          (er hard? 'expand-cp=>generate-type "Term is not a consp: ~q0"
-              term))
-         (fn (acl2::ffn-symb term))
-         ((unless (and fn (symbolp fn)))
-          (er hard? 'expand-cp=>generate-type "Term is not a function call: ~q0"
-              term))
-         (fc (is-function fn fn-lst))
-         ((unless fc)
-          (er hard? 'expand-cp=>generate-type "Function doesn't exist in the
-                       hint: ~q0" fn)))
-      (type-thm-full term fc state)))
+         (alst (pseudo-term-sym-alist-fix alst))
+         (clock (nfix clock))
+         (names (symbol-list-fix names))
+         ((unless (mbt (and (consp term)
+                            (pseudo-lambdap (car term))
+                            (not (zp clock)))))
+          (mv term alst names))
+         ((cons fncall actuals) term)
+         ((mv new-actuals alst-1 names-1)
+          (expand-term-list actuals hints fn-lvls alst clock names state))
+         ;; if a new-actual is a variable, then don't generate a new one
+         ((mv actual-vars alst-2 names-2)
+          (new-vars-for-actuals new-actuals alst-1 names-1))
+         (formals (lambda-formals fncall))
+         (body (lambda-body fncall))
+         (substed-body
+          (acl2::substitute-into-term body (pairlis$ formals actual-vars)))
+         ((mv new-body alst-3 names-3)
+          (expand-term substed-body hints fn-lvls alst-2
+                       (1- clock) names-2 state))
+         ((if (acl2::variablep new-body)) (mv new-body alst-3 names-3))
+         (body-var (new-fresh-var names-3)))
+      (mv body-var
+          (acons new-body body-var alst-3)
+          (cons body-var names-3))))
 
-  (defthm generate-type-correct
-    (implies (and (ev-smtcp-meta-extract-global-facts)
-                  (pseudo-termp term)
-                  (alistp a)
-                  (generate-type term fn-lst state))
-             (ev-smtcp (generate-type term fn-lst state) a))
-    :hints (("Goal"
-             :in-theory (e/d (generate-type)
-                             (type-thm-full-correct))
-             :use ((:instance
-                    type-thm-full-correct
-                    (term term)
-                    (func (is-function (car term)
-                                       (smt-function-list-fix fn-lst)))
-                    (state state)
-                    ))
-             ))
+  (define expand-fncall ((term pseudo-termp)
+                         (hints smtlink-hint-p)
+                         (fn-lvls sym-int-alistp)
+                         (alst pseudo-term-sym-alistp)
+                         (clock natp)
+                         (names symbol-listp)
+                         state)
+    :guard (and (consp term)
+                (symbolp (car term))
+                (not (equal (car term) 'quote))
+                (not (zp clock)))
+    :measure (list (nfix clock)
+                   (acl2-count (pseudo-term-fix term))
+                   1)
+    :returns (mv (new-term pseudo-termp)
+                 (new-alst pseudo-term-sym-alistp)
+                 (new-names symbol-listp))
+    (b* ((term (pseudo-term-fix term))
+         (hints (smtlink-hint-fix hints))
+         ((smtlink-hint h) hints)
+         (alst (pseudo-term-sym-alist-fix alst))
+         (clock (nfix clock))
+         (names (symbol-list-fix names))
+         ((unless (mbt (and (consp term)
+                            (symbolp (car term))
+                            (not (equal (car term) 'quote))
+                            (not (zp clock)))))
+          (mv term alst names))
+         ((cons fncall actuals) term)
+         ((mv new-actuals alst-1 names-1)
+          (expand-term-list actuals hints fn-lvls alst clock names state))
+         ((mv actual-vars alst-2 names-2)
+          (new-vars-for-actuals new-actuals alst-1 names-1))
+         (basic-function (member-equal fncall (SMT-basics)))
+         (flex? (fncall-of-fixtypes fncall h.types-info))
+         (lvl (assoc-equal fncall fn-lvls))
+         (user-defined (is-function fncall h.functions))
+         ;; There are three cases:
+         ;; 1. fn is a basic function (including fty functions), just return;
+         ;; 2. fn exists in fn-lvls, its level reaches 0, then just leave it
+         ;; there;
+         ;; 3. fn exists in fn-lvls, its level is not 0, then expand for 1;
+         ;; 4. the user wants to expand the function for 0 levels;
+         ;; 5. otherwise, expand for 1 level
+         ((if (or basic-function flex?
+                  (and lvl (<= (cdr lvl) 0))
+                  (and (not lvl)
+                       user-defined
+                       (<= (smt-function->expansion-depth user-defined) 0))))
+          (mv `(,fncall ,@new-actuals) alst-2 names-2))
+         ((mv formals body) (get-formals-body fncall state))
+         (substed-body
+          (acl2::substitute-into-term body (pairlis$ formals actual-vars)))
+         (new-lvls (update-fn-lvls fncall user-defined fn-lvls))
+         ((mv new-body alst-3 names-3)
+          (expand-term substed-body hints new-lvls alst-2
+                       (1- clock) names-2 state))
+         ((if (acl2::variablep new-body)) (mv new-body alst-3 names-3))
+         (body-var (new-fresh-var names-3)))
+      (mv body-var
+          (acons new-body body-var alst-3)
+          (cons body-var names-3)))
     )
 
-  (define compose-goal ((cl pseudo-term-listp)
-                        (to-be-learnt pseudo-term-listp)
-                        (fn-lst smt-function-list-p)
-                        state)
-    :returns (new-goal pseudo-term-listp)
-    :measure (len (pseudo-term-list-fix to-be-learnt))
-    (b* ((cl (pseudo-term-list-fix cl))
-         (to-be-learnt (pseudo-term-list-fix to-be-learnt))
-         ((unless (consp to-be-learnt)) cl)
-         ((cons first-fact rest-facts) to-be-learnt)
-         ((unless (and (not (acl2::variablep first-fact))
-                       (not (acl2::fquotep first-fact))
-                       (symbolp (car first-fact))))
-          cl)
-         (learnt-fact (transform (function-substitution first-fact state)))
-         (learnt-type (generate-type first-fact fn-lst state))
-         ((if (null learnt-fact)) cl)
-         ((if (null learnt-type)) cl))
-      `((not ,learnt-type)
-        (not ,learnt-fact)
-        ,@(compose-goal cl rest-facts fn-lst state))))
+  (define expand-term ((term pseudo-termp)
+                       (hints smtlink-hint-p)
+                       (fn-lvls sym-int-alistp)
+                       (alst pseudo-term-sym-alistp)
+                       (clock natp)
+                       (names symbol-listp)
+                       state)
+    :measure (list (nfix clock)
+                   (acl2-count (pseudo-term-fix term))
+                   2)
+    :returns (mv (new-term pseudo-termp)
+                 (new-alst pseudo-term-sym-alistp)
+                 (new-names symbol-listp))
+    (b* ((term (pseudo-term-fix term))
+         (alst (pseudo-term-sym-alist-fix alst))
+         (clock (nfix clock))
+         (names (symbol-list-fix names))
+         ((if (zp clock)) (mv term alst names))
+         (exist? (assoc-equal term alst))
+         ((if exist?) (mv (cdr exist?) alst names))
+         ((if (acl2::variablep term)) (mv term alst names))
+         ((if (acl2::quotep term)) (mv term alst names))
+         ((cons fn &) term)
+         ((if (pseudo-lambdap fn))
+          (expand-lambda term hints fn-lvls alst clock names state)))
+      (expand-fncall term hints fn-lvls alst clock names state)))
 
-  (encapsulate ()
-    (local (in-theory (e/d (compose-goal) ())))
-
-    (defthm compose-goal-correct
-      (implies (and (ev-smtcp-meta-extract-global-facts)
-                    (pseudo-term-listp clause)
-                    (alistp a)
-                    (ev-smtcp (disjoin
-                               (compose-goal clause to-be-learnt fn-lst state))
-                              a))
-               (ev-smtcp (disjoin clause) a))
-      :hints (("Goal"
-               :expand (compose-goal clause to-be-learnt fn-lst state)
-               :in-theory (e/d ()
-                               (ev-smtcp-of-disjoin
-                                transform-pseudo-termp))
-               :use
-               ((:instance transform-pseudo-termp
-                           (term (function-substitution
-                                  (car (pseudo-term-list-fix to-be-learnt))
-                                  state))
-                           (a a))))))
-
-    (defthm compose-transformed-goal-correct
-      (implies (and (ev-smtcp-meta-extract-global-facts)
-                    (pseudo-term-listp clause)
-                    (alistp a)
-                    (ev-smtcp
-                     (disjoin
-                      (compose-goal (transform-list clause)
-                                    to-be-learnt fn-lst state))
-                     a))
-               (ev-smtcp (disjoin clause) a)))
-    )
-
-  (encapsulate ()
-    (local
-     (defthm pseudo-term-listp-of-strip-cars-of-fact-alistp
-       (implies (fact-alistp x)
-                (pseudo-term-listp (strip-cars x)))))
-
-    (define expand-cp-helper ((cl pseudo-term-listp)
-                              (smtlink-hint t)
-                              state)
-      ;; :returns (new-goal pseudo-term-listp)
-      (b* (((unless (pseudo-term-listp cl)) (mv nil nil))
-           ((unless (smtlink-hint-p smtlink-hint))
-            (mv cl nil))
-           ((smtlink-hint h) smtlink-hint)
-           (fn-lst h.functions)
-           (fn-lvls (initialize-fn-lvls fn-lst))
-           (wrld-fn-len h.wrld-fn-len)
-           (transformed-cl (transform-list cl))
-           ;; Do function expansion
-           (to-be-learnt
-            (expand (disjoin transformed-cl)
-                    (make-ex-args
-                     :fn-lvls fn-lvls
-                     :fn-lst fn-lst
-                     :facts nil
-                     :fixinfo h.types-info
-                     :wrld-fn-len wrld-fn-len)
-                    state))
-           (expanded-goal (compose-goal transformed-cl
-                                        (strip-cars to-be-learnt) fn-lst
-                                        state))
-           (next-cp (cdr (assoc-equal 'expand *SMT-architecture*)))
-           ((if (null next-cp)) (mv cl nil))
-           (the-hint
-            `(:clause-processor (,next-cp clause ',h)))
-           (hinted-goal `((hint-please ',the-hint) ,@expanded-goal)))
-        (mv hinted-goal (strip-cars to-be-learnt))))
-    )
-
-  (defthm expand-cp-helper-correct
-    (implies (and (ev-smtcp-meta-extract-global-facts)
-                  (pseudo-term-listp cl)
-                  (alistp a)
-                  (ev-smtcp
-                   (disjoin
-                    (mv-nth 0 (expand-cp-helper cl hint state)))
-                   a))
-             (ev-smtcp (disjoin cl) a))
-    :hints (("Goal"
-             :in-theory (e/d (expand-cp-helper) (ev-smtcp-of-disjoin)))))
-
-  (define expand-cp-generalize ((cl pseudo-term-listp)
-                                (smtlink-hint t)
-                                state)
-    ;; :returns (subgoal-lst pseudo-term-list-listp)
-    :verify-guards nil
-    (b* (((mv hinted-goal to-be-learnt)
-          (expand-cp-helper cl smtlink-hint state))
-         ((unless (pseudo-term-listp hinted-goal))
-          (prog2$ (er hard? 'expand-cp=>expand-cp-generalize "Return type of
-                              expand-cp-helper is not pseudo-term-listp.~%")
-                  (list cl)))
-         (generalize-hint (list to-be-learnt 'x)))
-      (acl2::generalize-termlist-cp hinted-goal generalize-hint))
-    ///
-    (define expand-cp-alist ((cl pseudo-term-listp)
-                             (smtlink-hint t)
-                             state a)
-      :verify-guards nil
-      (b* (((mv hinted-goal to-be-learnt)
-            (expand-cp-helper cl smtlink-hint state))
-           ((unless (pseudo-term-listp hinted-goal))
-            (prog2$ (er hard? 'expand-cp=>expand-cp-alist "Return type of
-                              expand-cp-helper is not pseudo-term-listp.~%")
-                    a))
-           (generalize-hint (list to-be-learnt 'x)))
-        (generalize-termlist-alist hinted-goal generalize-hint a))
-      ))
-
-  (defthm expand-cp-generalize-correct
-    (implies (and (ev-smtcp-meta-extract-global-facts)
-                  (pseudo-term-listp cl)
-                  (alistp a)
-                  (ev-smtcp
-                   (conjoin-clauses (expand-cp-generalize cl hint state))
-                   (expand-cp-alist cl hint state a)))
-             (ev-smtcp (disjoin cl) a))
-    :hints (("Goal"
-             :do-not-induct t
-             :in-theory (e/d (expand-cp-generalize expand-cp-alist)
-                             (acl2::generalize-termlist-alist
-                              generalize-termlist-cp-correct-expand
-                              ev-smtcp-of-disjoin))
-             :use ((:instance generalize-termlist-cp-correct-expand
-                              (clause (mv-nth 0 (expand-cp-helper cl hint state)))
-                              (acl2::hint (cons (mv-nth 1 (expand-cp-helper cl hint state))
-                                                '(x)))
-                              (acl2::env a)))
-             )))
-
-  (define expand-cp ((cl pseudo-term-listp)
-                     (hints t)
-                     state)
-    :verify-guards nil
-    (b* ((expanded-clause (expand-cp-generalize cl hints state)))
-      (value expanded-clause)))
-
-  (defthm correctness-of-expand-cp
-    (implies (and (ev-smtcp-meta-extract-global-facts)
-                  (pseudo-term-listp cl)
-                  (alistp a)
-                  (ev-smtcp
-                   (conjoin-clauses
-                    (acl2::clauses-result
-                     (expand-cp cl hint state)))
-                   (expand-cp-alist cl hint state a)))
-             (ev-smtcp (disjoin cl) a))
-    :hints (("Goal"
-             :in-theory (disable ev-smtcp-of-disjoin)
-             :expand ((expand-cp cl hint state))))
-    :rule-classes :clause-processor)
+  (define expand-term-list ((term-lst pseudo-term-listp)
+                            (hints smtlink-hint-p)
+                            (fn-lvls sym-int-alistp)
+                            (alst pseudo-term-sym-alistp)
+                            (clock natp)
+                            (names symbol-listp)
+                            state)
+    :measure (list (nfix clock)
+                   (acl2-count (pseudo-term-list-fix term-lst))
+                   0)
+    :returns (mv (new-term-lst pseudo-term-listp)
+                 (new-alst pseudo-term-sym-alistp)
+                 (new-names symbol-listp))
+    (b* ((term-lst (pseudo-term-list-fix term-lst))
+         (alst (pseudo-term-sym-alist-fix alst))
+         (clock (nfix clock))
+         (names (symbol-list-fix names))
+         ((unless (consp term-lst)) (mv nil alst names))
+         ((cons term-hd term-tl) term-lst)
+         ((mv new-hd alst-1 names-1)
+          (expand-term term-hd hints fn-lvls alst clock names state))
+         ((mv new-tl alst-2 names-2)
+          (expand-term-list term-tl hints fn-lvls alst-1 clock names-1 state)))
+      (mv (cons new-hd new-tl) alst-2 names-2)))
   )
+)
+
+(defthm crock2
+  (alistp (pairlis$ x y)))
+
+(verify-guards expand-term
+  :hints (("Goal"
+           :in-theory (e/d ()
+                           ((:executable-counterpart smt-basics)
+                            pseudo-term-listp-of-symbol-listp
+                            member-equal
+                            symbolp-of-car-when-member-equal-of-sym-int-alistp
+                            acl2::symbol-listp-when-not-consp
+                            symbolp-of-fn-call-of-pseudo-termp
+                            pseudo-term-listp-of-cdr-pseudo-termp-if
+                            symbolp-of-caar-when-sym-int-alistp
+                            type-decl-p-definition
+                            acl2::pseudo-term-listp-cdr
+                            assoc-equal-of-sym-int-alist))
+           :use ((:instance assoc-equal-of-sym-int-alist
+                            (x (car term))
+                            (y fn-lvls))))))
